src/Bedrock/Group/ScalarMult/LadderStep.v
@@ -54,7 +54,7 @@ Section __.
 
   Instance spec_of_ladderstep : spec_of "ladderstep" :=
     fnspec! "ladderstep"
-          (pX1 pX2 pZ2 pX3 pZ3 : Semantics.word)
+          (pX1 pX2 pZ2 pX3 pZ3 : word)
           / (X1 X2 Z2 X3 Z3 : F M_pos) R,
     { requires tr mem :=
         (FElem (Some tight_bounds) pX1 X1
@@ -74,7 +74,7 @@ Section __.
               * FElem (Some tight_bounds) pX3 X5
               * FElem (Some tight_bounds) pZ3 Z5 * R)%sep mem'}.
 
-  Lemma compile_ladderstep {tr mem locals functions}
+  Lemma compile_ladderstep {tr m l functions}
         (x1 x2 z2 x3 z3 : F M_pos) :
     let v := ladderstep_gallina x1 x2 z2 x3 z3 in
     forall {P} {pred: P v -> predicate} {k: nlet_eq_k P v} {k_impl}
@@ -86,33 +86,33 @@ Section __.
 
       (FElem (Some tight_bounds) X1_ptr x1
        * FElem (Some tight_bounds) X2_ptr x2 * FElem (Some tight_bounds) Z2_ptr z2
-       * FElem (Some tight_bounds) X3_ptr x3 * FElem (Some tight_bounds) Z3_ptr z3 * Rout)%sep mem ->
+       * FElem (Some tight_bounds) X3_ptr x3 * FElem (Some tight_bounds) Z3_ptr z3 * Rout)%sep m ->
 
-        map.get locals X1_var = Some X1_ptr ->
-        map.get locals X2_var = Some X2_ptr ->
-        map.get locals Z2_var = Some Z2_ptr ->
-        map.get locals X3_var = Some X3_ptr ->
-        map.get locals Z3_var = Some Z3_ptr ->
+        map.get l X1_var = Some X1_ptr ->
+        map.get l X2_var = Some X2_ptr ->
+        map.get l Z2_var = Some Z2_ptr ->
+        map.get l X3_var = Some X3_ptr ->
+        map.get l Z3_var = Some Z3_ptr ->
 
         (let v := v in
-         forall X4 Z4 X5 Z5 (* output values *) m
+         forall X4 Z4 X5 Z5 (* output values *) m'
                 (Heq : ladderstep_gallina x1 x2 z2 x3 z3
                        = (X4, Z4, X5, Z5)),
           (FElem (Some tight_bounds) X1_ptr x1
            * FElem (Some tight_bounds) X2_ptr X4
            * FElem (Some tight_bounds) Z2_ptr Z4
            * FElem (Some tight_bounds) X3_ptr X5
-           * FElem (Some tight_bounds) Z3_ptr Z5 * Rout)%sep m ->
+           * FElem (Some tight_bounds) Z3_ptr Z5 * Rout)%sep m' ->
            (<{ Trace := tr;
-               Memory := m;
-               Locals := locals;
+               Memory := m';
+               Locals := l;
                Functions := functions }>
             k_impl
             <{ pred (k v eq_refl) }>)) ->
 
         <{ Trace := tr;
-           Memory := mem;
-           Locals := locals;
+           Memory := m;
+           Locals := l;
            Functions := functions }>
         cmd.seq
           (cmd.call [] "ladderstep"
@@ -167,6 +167,7 @@ Section __.
 
     
     Hint Immediate relax_bounds_FElem : ecancel_impl.
+    Hint Immediate drop_bounds_FElem : ecancel_impl.
 
 
     Ltac ecancel_assumption ::=  ecancel_assumption_impl.
